thys/examples/sorting/Sorting_Export_Code.thy
@@ -1,5 +1,5 @@
 theory Sorting_Export_Code
-imports (* Sorting_PDQ *) Sorting_Introsort (* Sorting_Strings *) Sorting_Results
+imports (* Sorting_PDQ *) Sorting_Introsort Sorting_Strings Sorting_Results
 begin
   
 text \<open>
@@ -34,6 +34,48 @@ lemmas [llvm_inline] = unat_sort.introsort_aux_impl_def
                       unat_sort.is_unguarded_insert_impl_def
 export_llvm "unat_sort_introsort_impl :: 64 word ptr \<Rightarrow> _" is "uint64_t* introsort(uint64_t*, int64_t,int64_t)"
   file "../code/introsort.ll"
+
+
+
+
+
+global_interpretation string_sort: sort_impl_context "(\<le>)" "(<)" "TYPE(64)" strcmp_impl
+              "string_cmp_cost n" "bstring_assn n TYPE(64) TYPE('w::len2)"
+  defines string_sort_is_guarded_insert_impl = string_sort.is_guarded_insert_impl
+      and string_sort_is_unguarded_insert_impl = string_sort.is_unguarded_insert_impl
+      and string_sort_unguarded_insertion_sort_impl = string_sort.unguarded_insertion_sort_impl
+      and string_sort_guarded_insertion_sort_impl = string_sort.guarded_insertion_sort_impl
+      and string_sort_final_insertion_sort_impl = string_sort.final_insertion_sort_impl
+      and string_sort_sift_down_impl   = string_sort.sift_down_impl
+      and string_sort_heapify_btu_impl = string_sort.heapify_btu_impl
+      and string_sort_heapsort_impl    = string_sort.heapsort_impl
+      and string_sort_qsp_next_l_impl       = string_sort.qsp_next_l_impl
+      and string_sort_qsp_next_h_impl       = string_sort.qsp_next_h_impl
+      and string_sort_qs_partition_impl     = string_sort.qs_partition_impl
+      and string_sort_partition_pivot_impl  = string_sort.partition_pivot_impl 
+      and string_sort_introsort_aux_impl = string_sort.introsort_aux_impl
+      and string_sort_move_median_to_first_impl = string_sort.move_median_to_first_impl
+      and string_sort_introsort_impl        = string_sort.introsort_impl  
+
+  apply (rule strcmp_sort_impl_context)
+  by simp
+
+
+lemma cheat[llvm_code,llvm_inline]: "(strcmp_impl :: 'w word ptr \<times> 'size_t word \<times> 'size_t word
+   \<Rightarrow> 'w word ptr \<times> 'size_t word \<times> 'size_t word
+      \<Rightarrow> 1 word llM) a v = return 1"
+  sorry
+lemmas [llvm_inline] = string_sort.introsort_aux_impl_def 
+                      string_sort.final_insertion_sort_impl_def
+                      string_sort.guarded_insertion_sort_impl_def
+                      string_sort.unguarded_insertion_sort_impl_def
+                      string_sort.is_guarded_insert_impl_def
+                      string_sort.is_unguarded_insert_impl_def 
+export_llvm   "string_sort_introsort_impl :: (8 word ptr \<times> 64 word \<times> 64 word) ptr \<Rightarrow> _" is "llstring* str_introsort(llstring*, int64_t, int64_t)"
+ defines \<open>typedef struct {char *data; struct {int64_t size; int64_t capacity;};} llstring;\<close> (*
+  file "../code/string_introsort.ll"
+*)
+
 
 
 end
